specs/lib/Spec.Lib.Endian.fsti
@@ -5,8 +5,11 @@ open Spec.Lib.IntTypes
 open FStar.HyperStack.ST
 
 inline_for_extraction
-val uint32_from_bytes_le: i:lbuffer uint8 4 -> Stack uint32 
+val uint32_from_bytes_le: i:lbuffer uint8 4 -> Stack uint32
 			 (requires (fun h -> live h i))
 			 (ensures (fun h0 _ h1 -> preserves_live h0 h1 /\ h0 == h1))
 
-
+inline_for_extraction
+val uint32_to_bytes_le: o:lbuffer uint8 4 -> uint32 -> Stack unit
+			 (requires (fun h -> live h o))
+			 (ensures (fun h0 _ h1 -> preserves_live h0 h1 /\ modifies1 o h0 h1))
